Added requires HasNext() to Next()
And a test!

src/StandardLibrary/Collections.dfy
@@ -2,152 +2,148 @@
 include "../StandardLibrary/StandardLibrary.dfy"
 include "../StandardLibrary/UInt.dfy"
 
-import opened StandardLibrary
-import opened UInt = StandardLibrary.UInt
 
-trait ByteProducer {
-  predicate Valid() reads this
-  predicate method HasNext()
-    requires Valid() 
-    ensures Valid()
-    reads this
-  method Next() returns (res: Option<uint8>)
-    requires Valid()
-    ensures Valid()
-    ensures HasNext() ==> res.Some? 
-    modifies this
 
-  method ForEachRemaining(consumer: ByteConsumer)
-    requires Valid()
-    ensures Valid()
-    modifies this, consumer
+module Collections {
+  import opened StandardLibrary
+  import opened UInt = StandardLibrary.UInt
+
+  trait ByteProducer {
+    predicate Valid() reads this
+    predicate method HasNext()
+      requires Valid() 
+      ensures Valid()
+      reads this
+    method Next() returns (res: uint8)
+      requires Valid()
+      requires HasNext()
+      ensures Valid()
+      modifies this
+
+    method ForEachRemaining(consumer: ByteConsumer)
+      requires Valid()
+      ensures Valid()
+      modifies this, consumer
+      decreases *
+    method TryForEachRemaining(consumer: ByteConsumer) returns (consumed: int)
+      requires Valid()
+      ensures Valid()
+      modifies this, consumer
+      decreases *
+  }
+
+  trait ByteConsumer {
+    predicate method CanAccept()
+    method Accept(b: uint8) returns (res: bool)
+  }
+
+  method DefaultForEachRemaining(producer: ByteProducer, consumer: ByteConsumer)
+    requires producer.Valid()
+    ensures producer.Valid()
+    modifies producer, consumer
     decreases *
-  method TryForEachRemaining(consumer: ByteConsumer) returns (consumed: int)
-    requires Valid()
-    ensures Valid()
-    modifies this, consumer
-    decreases *
-}
-
-trait ByteConsumer {
-  predicate method CanAccept()
-  method Accept(b: uint8) returns (res: bool)
-}
-
-method DefaultForEachRemaining(producer: ByteProducer, consumer: ByteConsumer)
-  requires producer.Valid()
-  ensures producer.Valid()
-  modifies producer, consumer
-  decreases *
-{
-  while producer.HasNext() 
-    invariant producer.Valid()
-    decreases * 
   {
-    var byte := producer.Next();
-    // TODO-RS: Dafny isn't convinced this is always true for some reason
-    if byte.Some? {
-      var _ := consumer.Accept(byte.get);
+    while producer.HasNext() 
+      invariant producer.Valid()
+      decreases * 
+    {
+      var byte := producer.Next();
+      var _ := consumer.Accept(byte);
     }
   }
-}
 
-method DefaultTryForEachRemaining(producer: ByteProducer, consumer: ByteConsumer) returns (consumed: int) 
-  requires producer.Valid()
-  ensures producer.Valid()
-  modifies producer, consumer
-  decreases *
-{
-  consumed := 0;
-  while producer.HasNext() && consumer.CanAccept()
-    invariant producer.Valid()
-    decreases * 
+  method DefaultTryForEachRemaining(producer: ByteProducer, consumer: ByteConsumer) returns (consumed: int) 
+    requires producer.Valid()
+    ensures producer.Valid()
+    modifies producer, consumer
+    decreases *
   {
-    var byte := producer.Next();
-    // TODO-RS: Dafny isn't convinced this is always true for some reason
-    if byte.Some? {
-      var _ := consumer.Accept(byte.get);
+    consumed := 0;
+    while producer.HasNext() && consumer.CanAccept()
+      invariant producer.Valid()
+      decreases * 
+    {
+      var byte := producer.Next();
+      var _ := consumer.Accept(byte);
+      consumed := consumed + 1;
     }
-    consumed := consumed + 1;
   }
-}
 
-class ArrayByteProducer extends ByteProducer {
-  const bytes: array<uint8>
-  var index: int
-  var maxIndex: int
-  predicate Valid() reads this {
-    0 <= index <= maxIndex <= bytes.Length
-  }
-  predicate method HasNext() reads this requires Valid() ensures Valid() {
-    index < maxIndex
-  }
-  method Next() returns (res: Option<uint8>) 
-    requires Valid()
-    ensures Valid()
-    ensures HasNext() ==> res.Some? 
-    modifies this
-  {
-    if index >= maxIndex {
-      res := None;
-    } else {
-      res := Some(bytes[index]);
+  class ArrayByteProducer extends ByteProducer {
+    const bytes: array<uint8>
+    var index: int
+    var maxIndex: int
+    predicate Valid() reads this {
+      0 <= index <= maxIndex <= bytes.Length
+    }
+    constructor(bytes: array<uint8>) 
+      ensures Valid()
+    {
+      this.bytes := bytes;
+      this.index := 0;
+      this.maxIndex := bytes.Length;
+    }
+    predicate method HasNext() reads this requires Valid() ensures Valid() {
+      index < maxIndex
+    }
+    method Next() returns (res: uint8) 
+      requires Valid()
+      requires HasNext()
+      ensures Valid()
+      modifies this
+    {
+      res := bytes[index];
       index := index + 1;
     }
-  }
-  method ForEachRemaining(consumer: ByteConsumer) 
-    requires Valid()
-    ensures Valid()
-    modifies this, consumer
-    decreases *
-  {
-    DefaultForEachRemaining(this, consumer);
-  }
-  method TryForEachRemaining(consumer: ByteConsumer) returns (consumed: int) 
-    requires Valid()
-    ensures Valid()
-    modifies this, consumer
-    decreases *
-  {
-    consumed := DefaultTryForEachRemaining(this, consumer);
-  }
-}
-
-class SequenceByteProducer extends ByteProducer {
-  var bytesRemaining: seq<uint8>
-  predicate Valid() reads this {
-    true
-  }
-  predicate method HasNext() reads this {
-    |bytesRemaining| > 0
-  }
-  method Next() returns (res: Option<uint8>)
-    requires Valid()
-    ensures Valid()
-    ensures HasNext() ==> res.Some? 
-    modifies this
-  {
-    if |bytesRemaining| == 0 {
-      res := None;
-    } else {
-      res := Some(bytesRemaining[0]);
-      bytesRemaining := bytesRemaining[1..];
+    method ForEachRemaining(consumer: ByteConsumer) 
+      requires Valid()
+      ensures Valid()
+      modifies this, consumer
+      decreases *
+    {
+      DefaultForEachRemaining(this, consumer);
+    }
+    method TryForEachRemaining(consumer: ByteConsumer) returns (consumed: int) 
+      requires Valid()
+      ensures Valid()
+      modifies this, consumer
+      decreases *
+    {
+      consumed := DefaultTryForEachRemaining(this, consumer);
     }
   }
-  method ForEachRemaining(consumer: ByteConsumer) 
-    requires Valid()
-    ensures Valid()
-    modifies this, consumer
-    decreases *
-  {
-    DefaultForEachRemaining(this, consumer);
-  }
-  method TryForEachRemaining(consumer: ByteConsumer) returns (consumed: int) 
-    requires Valid()
-    ensures Valid()
-    modifies this, consumer
-    decreases *
-  {
-    consumed := DefaultTryForEachRemaining(this, consumer);
+
+  class SequenceByteProducer extends ByteProducer {
+    var bytesRemaining: seq<uint8>
+    predicate Valid() reads this {
+      true
+    }
+    predicate method HasNext() reads this {
+      |bytesRemaining| > 0
+    }
+    method Next() returns (res: uint8)
+      requires Valid()
+      requires HasNext()
+      modifies this
+    {
+      res := bytesRemaining[0];
+      bytesRemaining := bytesRemaining[1..];
+    }
+    method ForEachRemaining(consumer: ByteConsumer) 
+      requires Valid()
+      ensures Valid()
+      modifies this, consumer
+      decreases *
+    {
+      DefaultForEachRemaining(this, consumer);
+    }
+    method TryForEachRemaining(consumer: ByteConsumer) returns (consumed: int) 
+      requires Valid()
+      ensures Valid()
+      modifies this, consumer
+      decreases *
+    {
+      consumed := DefaultTryForEachRemaining(this, consumer);
+    }
   }
 }
