test/StandardLibrary/Collections.dfy
@@ -1,0 +1,34 @@
+
+include "../../src/StandardLibrary/StandardLibrary.dfy"
+include "../../src/StandardLibrary/UInt.dfy"
+include "../../src/StandardLibrary/Collections.dfy"
+
+module CollectionsTests {
+  import opened StandardLibrary
+  import opened UInt = StandardLibrary.UInt
+  import opened Collections
+
+  method {:test} ArrayByteProducer() {
+    var bytes := new uint8[5];
+    bytes[0] := 1;
+    bytes[1] := 2;
+    bytes[2] := 3;
+    bytes[3] := 4;
+    bytes[4] := 5;
+
+    var producer := new ArrayByteProducer(bytes);
+    expect producer.HasNext();
+    var byte := producer.Next();
+    expect byte == 1;
+  }
+
+  method ExpectNext(producer: ByteProducer, expected: uint8) 
+    requires producer.Valid()
+    ensures producer.Valid()
+    modifies producer
+  {
+    expect producer.HasNext();
+    var byte := producer.Next();
+    expect byte == 1;
+  }
+}
